Merkle trees serialization parameterization

secure_api/merkle_tree/MerkleTree.New.Low.Serialization.fst
@@ -26,6 +26,11 @@ module U32 = FStar.UInt32
 module U64 = FStar.UInt64
 module U8 = FStar.UInt8
 
+open MerkleTree.New.Low.Hashes
+open MerkleTree.New.Low.Datastructures
+open MerkleTree.New.Low.Hashfunctions
+module MTS = MerkleTree.Spec
+
 let uint8_t = U8.t
 let uint16_t = U16.t
 let uint32_t = U32.t
@@ -76,7 +81,9 @@ private let serialize_uint64_t (ok:bool) (x:uint64_t) (buf:uint8_p) (sz:uint32_t
 private let serialize_offset_t = serialize_uint64_t
 private let serialize_index_t = serialize_uint32_t
 
-private let rec serialize_hash_i (ok:bool) (x:hash) (buf:uint8_p) (sz:uint32_t{B.len buf = sz}) (pos:uint32_t) (i:uint32_t{i < hash_size})
+private let rec serialize_hash_i 
+  (#hash_size:hash_size_t) 
+  (ok:bool) (x:hash #hash_size) (buf:uint8_p) (sz:uint32_t{B.len buf = sz}) (pos:uint32_t) (i:uint32_t{i < hash_size})
 : HST.ST (bool & uint32_t)
     (requires (fun h0 -> B.live h0 buf /\ B.live h0 x /\ B.len x = hash_size))
     (ensures (fun h0 _ h1 -> modifies (B.loc_buffer buf) h0 h1))
@@ -84,21 +91,31 @@ private let rec serialize_hash_i (ok:bool) (x:hash) (buf:uint8_p) (sz:uint32_t{B
   else let b = x.(i) in
        let ok, pos = serialize_uint8_t ok (Lib.RawIntTypes.u8_to_UInt8 b) buf sz pos in
        let j = i + 1ul in
-       if j < hash_size then serialize_hash_i ok x buf sz pos j
+       if j < hash_size then serialize_hash_i #hash_size ok x buf sz pos j
        else (ok, pos)
 
 private
-let serialize_hash (ok:bool) (x:hash) (buf:uint8_p) (sz:uint32_t{B.len buf = sz}) (pos:uint32_t) : HST.ST (bool & uint32_t)
+let serialize_hash 
+  (#hash_size:hash_size_t) 
+  (ok:bool) (x:hash #hash_size) (buf:uint8_p) (sz:uint32_t{B.len buf = sz}) (pos:uint32_t) 
+: HST.ST (bool & uint32_t)
   (requires (fun h0 -> B.live h0 buf /\ B.live h0 x /\ B.len x = hash_size))
   (ensures (fun h0 _ h1 -> modifies (B.loc_buffer buf) h0 h1))
 = if not ok || pos >= sz then (false, 0ul)
   else serialize_hash_i ok x buf sz pos 0ul
 
+#push-options "--z3rlimit 200 --initial_fuel 1 --max_fuel 1"
 private inline_for_extraction unfold
-let hash_vec_bytes (v:hash_vec) = 4UL + U64.mul (u32_64 (V.size_of v)) (u32_64 hash_size)
+let hash_vec_bytes (#hash_size:hash_size_t) (v:hash_vec #hash_size) = 
+  let vs_hs = U64.mul (u32_64 (V.size_of v)) (u32_64 hash_size) in
+  if vs_hs > U64.uint_to_t ((pow2 64) - 5) then U64.uint_to_t ((pow2 64) - 1)
+  else 4UL + vs_hs
+#pop-options
 
 private
-let rec serialize_hash_vec_i (ok:bool) (x:hash_vec) (buf:uint8_p) (sz:uint32_t{B.len buf = sz}) (pos:uint32_t) (i:uint32_t{i < V.size_of x})
+let rec serialize_hash_vec_i 
+  (#hash_size:hash_size_t) 
+  (ok:bool) (x:hash_vec #hash_size) (buf:uint8_p) (sz:uint32_t{B.len buf = sz}) (pos:uint32_t) (i:uint32_t{i < V.size_of x})
 : HST.ST (bool & uint32_t)
   (requires (fun h0 -> B.live h0 buf /\ RV.rv_inv h0 x /\ loc_disjoint (B.loc_buffer buf) (loc_rvector x)))
   (ensures (fun h0 _ h1 -> RV.rv_inv h1 x /\ modifies (B.loc_buffer buf) h0 h1))
@@ -112,7 +129,10 @@ let rec serialize_hash_vec_i (ok:bool) (x:hash_vec) (buf:uint8_p) (sz:uint32_t{B
   end
 
 private
-let serialize_hash_vec (ok:bool) (x:hash_vec) (buf:uint8_p) (sz:uint32_t{B.len buf = sz}) (pos:uint32_t) : HST.ST (bool & uint32_t)
+let serialize_hash_vec 
+  (#hash_size:hash_size_t) 
+  (ok:bool) (x:hash_vec #hash_size) (buf:uint8_p) (sz:uint32_t{B.len buf = sz}) (pos:uint32_t) 
+: HST.ST (bool & uint32_t)
   (requires (fun h0 -> B.live h0 buf /\ RV.rv_inv h0 x /\ HS.disjoint (B.frameOf buf) (Rgl?.region_of hvreg x)))
   (ensures (fun h0 _ h1 -> RV.rv_inv h1 x /\ modifies (B.loc_buffer buf) h0 h1))
 = if not ok || pos >= sz then (false, 0ul)
@@ -125,28 +145,38 @@ let serialize_hash_vec (ok:bool) (x:hash_vec) (buf:uint8_p) (sz:uint32_t{B.len b
     else (ok, pos)
   end
 
+#push-options "--z3rlimit 200 --initial_fuel 1 --max_fuel 1"
 private inline_for_extraction
-let rec hash_vv_bytes_i (vv:hash_vv) (i:uint32_t): HST.ST uint64_t
-    (requires (fun h0 -> V.live h0 vv))
-    (ensures (fun h0 _ h1 -> h0 == h1))
-  = if i >= V.size_of vv then 4UL
-    else begin
-      let vvi = V.index vv i in
-      let r = hash_vec_bytes vvi in
-      let rest = hash_vv_bytes_i vv (i+1ul) in
-      if uint64_max - rest < r then uint64_max
-      else rest + r
-    end
+let rec hash_vv_bytes_i 
+  (#hash_size:hash_size_t) 
+  (vv:hash_vv #hash_size) (i:uint32_t)
+: HST.ST uint64_t
+  (requires (fun h0 -> V.live h0 vv))
+  (ensures (fun h0 _ h1 -> h0 == h1))
+= if i >= V.size_of vv then 4UL
+  else begin
+    let vvi = V.index vv i in
+    let r = hash_vec_bytes vvi in
+    let rest = hash_vv_bytes_i vv (i+1ul) in
+    if uint64_max - rest < r then uint64_max
+    else rest + r
+  end
+#pop-options
 
 private inline_for_extraction
-let hash_vv_bytes (vv:hash_vv{V.size_of vv = merkle_tree_size_lg}): HST.ST uint64_t
+let hash_vv_bytes 
+  (#hash_size:hash_size_t) 
+  (vv:hash_vv #hash_size {V.size_of vv = merkle_tree_size_lg})
+: HST.ST uint64_t
   (requires (fun h0 -> V.live h0 vv))
   (ensures (fun h0 _ h1 -> h0 == h1))
 = hash_vv_bytes_i vv 0ul
 
-#push-options "--initial_fuel 1 --max_fuel 1"
+#push-options "--z3rlimit 1000 --initial_fuel 1 --max_fuel 1 --initial_ifuel 1 --max_ifuel 1"
 private
-let rec serialize_hash_vv_i (ok:bool) (x:hash_vv) (buf:uint8_p) (sz:uint32_t{B.len buf = sz}) (pos:uint32_t) (i:uint32_t{i < V.size_of x})
+let rec serialize_hash_vv_i 
+  (#hash_size:hash_size_t) 
+  (ok:bool) (x:hash_vv #hash_size) (buf:uint8_p) (sz:uint32_t{B.len buf = sz}) (pos:uint32_t) (i:uint32_t{i < V.size_of x})
 : HST.ST (bool & uint32_t)
   (requires (fun h0 -> B.live h0 buf /\ RV.rv_inv h0 x /\ HS.disjoint (B.frameOf buf) (Rgl?.region_of hvvreg x)))
   (ensures (fun h0 _ h1 -> modifies (B.loc_buffer buf) h0 h1))
@@ -154,18 +184,20 @@ let rec serialize_hash_vv_i (ok:bool) (x:hash_vv) (buf:uint8_p) (sz:uint32_t{B.l
   else begin
     let vi = V.index x i in
     let h0 = HST.get() in
-    let ok, pos = serialize_hash_vec ok vi buf sz pos in
+    let ok, pos = serialize_hash_vec #hash_size ok vi buf sz pos in
     let h1 = HST.get() in
     let j = i + 1ul in
-    if j < V.size_of x then begin
-      serialize_hash_vv_i ok x buf sz pos j
-    end
+    if j < V.size_of x then
+      serialize_hash_vv_i #hash_size ok x buf sz pos j
     else (ok, pos)
   end
 #pop-options
 
 private
-let serialize_hash_vv (ok:bool) (x:hash_vv) (buf:uint8_p) (sz:uint32_t{B.len buf = sz}) (pos:uint32_t): HST.ST (bool & uint32_t)
+let serialize_hash_vv 
+  (#hash_size:hash_size_t) 
+  (ok:bool) (x:hash_vv #hash_size) (buf:uint8_p) (sz:uint32_t{B.len buf = sz}) (pos:uint32_t)
+: HST.ST (bool & uint32_t)
   (requires (fun h0 -> B.live h0 buf /\ RV.rv_inv h0 x /\ HS.disjoint (B.frameOf buf) (Rgl?.region_of hvvreg x)))
   (ensures (fun h0 _ h1 -> modifies (B.loc_buffer buf) h0 h1))
 = if not ok || pos >= sz then (false, 0ul)
@@ -229,7 +261,10 @@ private let deserialize_offset_t = deserialize_uint64_t
 private let deserialize_index_t = deserialize_uint32_t
 
 private
-let deserialize_hash (ok:bool) (buf:const_uint8_p) (sz:uint32_t{CB.length buf = U32.v sz}) (r:HST.erid) (pos:uint32_t): HST.ST (bool & uint32_t & hash)
+let deserialize_hash 
+  (#hash_size:hash_size_t) 
+  (ok:bool) (buf:const_uint8_p) (sz:uint32_t{CB.length buf = U32.v sz}) (r:HST.erid) (pos:uint32_t)
+: HST.ST (bool & uint32_t & hash #hash_size)
   (requires (fun h0 -> CB.live h0 buf))
   (ensures (fun h0 (k, _, h) h1 -> (k ==> Rgl?.r_inv hreg h1 h) /\
                                    loc_disjoint (loc_buffer (CB.cast buf)) (loc_buffer h) /\
@@ -243,7 +278,9 @@ let deserialize_hash (ok:bool) (buf:const_uint8_p) (sz:uint32_t{CB.length buf = 
   end
 
 private
-let rec deserialize_hash_vec_i (ok:bool) (buf:const_uint8_p) (sz:uint32_t{CB.length buf = U32.v sz}) (r:HST.erid) (pos:uint32_t) (res:hash_vec) (i:uint32_t{i < V.size_of res})
+let rec deserialize_hash_vec_i 
+  (#hash_size:hash_size_t) 
+  (ok:bool) (buf:const_uint8_p) (sz:uint32_t{CB.length buf = U32.v sz}) (r:HST.erid) (pos:uint32_t) (res:hash_vec #hash_size) (i:uint32_t{i < V.size_of res})
 : HST.ST (bool & uint32_t)
   (requires (fun h0 -> CB.live h0 buf /\ V.live h0 res))
   (ensures (fun h0 _ h1 -> B.modifies (B.loc_buffer (V.Vec?.vs res)) h0 h1))
@@ -272,7 +309,10 @@ let rec deserialize_hash_vec_i (ok:bool) (buf:const_uint8_p) (sz:uint32_t{CB.len
   end
 
 private
-let deserialize_hash_vec (ok:bool) (buf:const_uint8_p) (sz:uint32_t{CB.length buf = U32.v sz}) (r:HST.erid) (pos:uint32_t): HST.ST (bool & uint32_t & hash_vec)
+let deserialize_hash_vec 
+  (#hash_size:hash_size_t) 
+  (ok:bool) (buf:const_uint8_p) (sz:uint32_t{CB.length buf = U32.v sz}) (r:HST.erid) (pos:uint32_t)
+: HST.ST (bool & uint32_t & hash_vec #hash_size)
   (requires (fun h0 -> CB.live h0 buf))
   (ensures (fun h0 _ h1 -> B.modifies B.loc_none h0 h1))
 = if not ok || pos >= sz then (false, pos, Rgl?.dummy hvreg)
@@ -288,7 +328,9 @@ let deserialize_hash_vec (ok:bool) (buf:const_uint8_p) (sz:uint32_t{CB.length bu
   end
 
 private
-let rec deserialize_hash_vv_i (ok:bool) (buf:const_uint8_p) (sz:uint32_t{CB.length buf = U32.v sz}) (r:HST.erid) (pos:uint32_t) (res:hash_vv) (i:uint32_t{i < V.size_of res})
+let rec deserialize_hash_vv_i 
+  (#hash_size:hash_size_t) 
+  (ok:bool) (buf:const_uint8_p) (sz:uint32_t{CB.length buf = U32.v sz}) (r:HST.erid) (pos:uint32_t) (res:hash_vv #hash_size) (i:uint32_t{i < V.size_of res})
 : HST.ST (bool & uint32_t)
   (requires (fun h0 -> CB.live h0 buf /\ V.live h0 res /\
                        B.loc_disjoint (CB.loc_buffer buf) (V.loc_vector res)))
@@ -319,7 +361,10 @@ let rec deserialize_hash_vv_i (ok:bool) (buf:const_uint8_p) (sz:uint32_t{CB.leng
     end
   end
 
-private let deserialize_hash_vv (ok:bool) (buf:const_uint8_p) (sz:uint32_t{CB.length buf = U32.v sz}) (r:HST.erid) (pos:uint32_t): HST.ST (bool & uint32_t & hash_vv)
+private let deserialize_hash_vv 
+  (#hash_size:hash_size_t) 
+  (ok:bool) (buf:const_uint8_p) (sz:uint32_t{CB.length buf = U32.v sz}) (r:HST.erid) (pos:uint32_t)
+: HST.ST (bool & uint32_t & hash_vv #hash_size)
   (requires (fun h0 -> CB.live h0 buf))
   (ensures (fun h0 _ h1 -> modifies B.loc_none h0 h1))
 = if not ok || pos >= sz then (false, pos, V.alloc_empty hash_vec)
@@ -334,7 +379,7 @@ private let deserialize_hash_vv (ok:bool) (buf:const_uint8_p) (sz:uint32_t{CB.le
     end
   end
 
-#set-options "--z3rlimit 10"
+#push-options "--z3rlimit 10"
 val mt_serialize_size: mt:const_mt_p -> HST.ST uint64_t
   (requires (fun h0 -> mt_safe h0 (CB.cast mt)))
   (ensures (fun _ _ h1 -> mt_safe h1 (CB.cast mt)))
@@ -352,12 +397,12 @@ let mt_serialize_size mt =
     hs_sz +              // hs
     1UL +                // rhs_ok
     hash_vec_bytes rhs + // rhs
-    u32_64 hash_size     // mroot
+    u32_64 (MT?.hash_size mtv) // mroot
   else
     uint64_max
-#reset-options
+#pop-options
 
-#set-options "--z3rlimit 15"
+#push-options "--z3rlimit 15 --initial_fuel 1 --max_fuel 1"
 val mt_serialize: mt:const_mt_p -> output:uint8_p -> sz:uint64_t -> HST.ST uint64_t
   (requires (fun h0 -> mt_safe h0 (CB.cast mt) /\ B.live h0 output /\ B.length output = U64.v sz /\
                        HS.disjoint (B.frameOf output) (B.frameOf (CB.cast mt))))
@@ -369,7 +414,7 @@ let mt_serialize mt output sz =
   let h0 = HST.get() in
   let ok, pos = serialize_uint8_t true 0uy output sz 0ul in // format version = 0uy
   let h1 = HST.get() in mt_safe_preserved mt (B.loc_buffer output) h0 h1;
-  let ok, pos = serialize_uint32_t ok hash_size output sz pos in
+  let ok, pos = serialize_uint32_t ok (MT?.hash_size mtv) output sz pos in
   let h2 = HST.get() in mt_safe_preserved mt (B.loc_buffer output) h1 h2;
   let ok, pos = serialize_offset_t ok (MT?.offset mtv) output sz pos in
   let h3 = HST.get() in mt_safe_preserved mt (B.loc_buffer output) h2 h3;
@@ -387,16 +432,21 @@ let mt_serialize mt output sz =
   let h9 = HST.get() in mt_safe_preserved mt (B.loc_buffer output) h8 h9;
   if ok then (FStar.Int.Cast.uint32_to_uint64 pos) else 0UL
 
-val mt_deserialize: rid:HST.erid -> input:const_uint8_p -> sz:uint64_t{CB.length input = U64.v sz} -> HST.ST (B.pointer_or_null merkle_tree)
+val mt_deserialize: 
+  #hash_size:hash_size_t ->
+  rid:HST.erid -> input:const_uint8_p -> sz:uint64_t{CB.length input = U64.v sz} -> 
+  hash_spec:Ghost.erased(MTS.hash_fun_t #(U32.v hash_size)) -> hash_fun:hash_fun_t #hash_size #hash_spec 
+-> HST.ST (B.pointer_or_null merkle_tree)
   (requires (fun h0 -> CB.live h0 input /\ HS.disjoint rid (B.frameOf (CB.cast input))))
   (ensures (fun h0 r h1 -> modifies B.loc_none h0 h1))
-let mt_deserialize rid input sz =
+let mt_deserialize #hash_size rid input sz hash_spec hash_fun =
   let sz = FStar.Int.Cast.uint64_to_uint32 sz in
   let hrid = HST.new_region rid in
   let hvrid = HST.new_region rid in
   let hvvrid = HST.new_region rid in
   let ok, pos, format_version = deserialize_uint8_t true input sz 0ul in
-  let ok, pos, hash_size = deserialize_uint32_t ok input sz pos in
+  let ok, pos, hsz = deserialize_uint32_t ok input sz pos in
+  let ok = ok && hsz = hash_size in
   let ok, pos, offset = deserialize_offset_t ok input sz pos in
   let ok, pos, i = deserialize_index_t ok input sz pos in
   let ok, pos, j = deserialize_index_t ok input sz pos in
@@ -406,16 +456,18 @@ let mt_deserialize rid input sz =
   let ok, pos, mroot = deserialize_hash ok input sz hrid pos in
   begin
     if not ok ||
-       hash_size <> MerkleTree.New.Low.hash_size ||
+       hash_size <> hash_size ||
        not (merkle_tree_conditions offset i j hs rhs_ok rhs mroot)
     then B.null #merkle_tree
-    else B.malloc rid (MT offset i j hs rhs_ok rhs mroot hash_2) 1ul
+    else B.malloc rid (MT hash_size offset i j hs rhs_ok rhs mroot hash_spec hash_fun) 1ul
   end
 
-val mt_serialize_path: p:const_path_p -> mt:const_mt_p -> output:uint8_p -> sz:uint64_t -> HST.ST uint64_t
+val mt_serialize_path: #hsz:hash_size_t -> p:const_path_p #hsz -> mt:const_mt_p -> output:uint8_p -> sz:uint64_t -> HST.ST uint64_t
   (requires (fun h0 -> let ncp = CB.cast p in
                        let mt = CB.cast mt in
-                       let phv:hash_vec = B.get h0 ncp 0 in                       
+                       let mtv = B.get h0 mt 0 in
+                       let phv:hash_vec = B.get h0 ncp 0 in
+                       MT?.hash_size mtv = hsz /\
                        path_safe h0 (B.frameOf mt) ncp /\ RV.rv_inv h0 phv /\
                        mt_safe h0 mt /\
                        B.live h0 output /\ B.length output = U64.v sz /\
@@ -423,26 +475,29 @@ val mt_serialize_path: p:const_path_p -> mt:const_mt_p -> output:uint8_p -> sz:u
                        HH.disjoint (B.frameOf mt) (B.frameOf ncp)))
   (ensures (fun h0 _ h1 -> path_safe h1 (B.frameOf (CB.cast mt)) (CB.cast p) /\
                            modifies (B.loc_buffer output) h0 h1))
-let mt_serialize_path p mt output sz =
+let mt_serialize_path #hsz p mt output sz =
   let sz = FStar.Int.Cast.uint64_to_uint32 sz in
   let ncp = CB.cast p in
   let h0 = HST.get() in
-  let ok, pos = serialize_uint32_t true hash_size output sz 0ul in
+  let ok, pos = serialize_uint32_t true hsz output sz 0ul in
   let h1 = HST.get() in
   let ok, pos = serialize_hash_vec ok !*ncp output sz pos in
   if ok then (FStar.Int.Cast.uint32_to_uint64 pos) else 0UL
 
-val mt_deserialize_path: rid:HST.erid -> input:const_uint8_p -> sz:uint64_t{CB.length input = U64.v sz} -> HST.ST (B.pointer_or_null path)
+val mt_deserialize_path: 
+  #hsz:hash_size_t ->
+  rid:HST.erid -> input:const_uint8_p -> sz:uint64_t{CB.length input = U64.v sz}
+-> HST.ST (B.pointer_or_null (path #hsz))
   (requires (fun h0 -> CB.live h0 input /\ HS.disjoint rid (B.frameOf (CB.cast input))))
   (ensures (fun h0 r h1 -> modifies B.loc_none h0 h1))
-let mt_deserialize_path rid input sz =
+let mt_deserialize_path #hsz rid input sz =
   let sz = FStar.Int.Cast.uint64_to_uint32 sz in
   let hvvrid = HST.new_region rid in
   let ok, pos, hash_size = deserialize_uint32_t true input sz 0ul in
   let ok, pos, hs = deserialize_hash_vec ok input sz hvvrid pos in
   begin
-    if not ok || hash_size <> MerkleTree.New.Low.hash_size
+    if not ok || hash_size <> hsz
     then B.null #path
     else B.malloc rid hs 1ul
   end
-#reset-options
+#pop-options
